Changed invariant predicate.
Now that replicas can perform garbage collection when moving
the Working Window, we need to base the invariant on the messages
in the network, since the network is our arbiter that keeps all
messages indefinitely.

docs/sbft-formal-model/proof.dfy
@@ -173,6 +173,15 @@ module Proof {
                                          commitMsg.payload.seqID))
   }
 
+  predicate {:opaque} EveryCommitIsSupportedByPreviouslySentPrepares(c:Constants, v:Variables) {
+    && v.WF(c)
+    && (forall commitMsg | && commitMsg in v.network.sentMsgs
+                           && commitMsg.payload.Commit?
+                           && IsHonestReplica(c, commitMsg.sender)
+          :: QuorumOfPreparesInNetwork(c, v, commitMsg.payload.view, 
+                                       commitMsg.payload.seqID, commitMsg.payload.operationWrapper))
+  }
+
   predicate {:opaque} EveryCommitClientOpMatchesRecordedPrePrepare(c:Constants, v:Variables) {
     && v.WF(c)
     && (forall commitMsg | && commitMsg in v.network.sentMsgs
@@ -246,7 +255,7 @@ module Proof {
     && EveryCommitMsgIsSupportedByAQuorumOfPrepares(c, v)
     && RecordedPreparesClientOpsMatchPrePrepare(c, v)
     && RecordedCommitsClientOpsMatchPrePrepare(c, v)
-    && EveryCommitIsSupportedByRecordedPrepares(c, v)
+    && EveryCommitIsSupportedByPreviouslySentPrepares(c, v)
     && EveryCommitClientOpMatchesRecordedPrePrepare(c, v)
     && HonestReplicasLockOnPrepareForGivenView(c, v)
     && HonestReplicasLockOnCommitForGivenView(c, v)
@@ -430,7 +439,7 @@ module Proof {
     requires Inv(c, v)
     requires NextStep(c, v, v', step)
     ensures RecordedCommitsClientOpsMatchPrePrepare(c, v')
-    ensures EveryCommitIsSupportedByRecordedPrepares(c, v')
+    ensures EveryCommitIsSupportedByPreviouslySentPrepares(c, v')
     ensures EveryCommitClientOpMatchesRecordedPrePrepare(c, v')
     ensures HonestReplicasLockOnCommitForGivenView(c, v')
     ensures EveryCommitMsgIsSupportedByAQuorumOfPrepares(c, v')
@@ -438,7 +447,7 @@ module Proof {
   {
     ProofEveryCommitMsgIsSupportedByAQuorumOfPrepares(c, v, v', step);
     reveal_RecordedCommitsClientOpsMatchPrePrepare();
-    reveal_EveryCommitIsSupportedByRecordedPrepares();
+    reveal_EveryCommitIsSupportedByPreviouslySentPrepares();
     reveal_EveryCommitClientOpMatchesRecordedPrePrepare();
     reveal_HonestReplicasLockOnCommitForGivenView();
     ProofCommitMsgsFromHonestSendersAgree(c, v, v', step);
@@ -1036,7 +1045,7 @@ module Proof {
   {
     if Init(c, v) {
       reveal_RecordedCommitsClientOpsMatchPrePrepare();
-      reveal_EveryCommitIsSupportedByRecordedPrepares();
+      reveal_EveryCommitIsSupportedByPreviouslySentPrepares();
       reveal_EveryCommitClientOpMatchesRecordedPrePrepare();
       reveal_HonestReplicasLockOnCommitForGivenView();
       reveal_CommitMsgsFromHonestSendersAgree();
